started with system validation

Mt/System/Validation.lean
@@ -1,5 +1,6 @@
 import Mt.System.Basic
 import Mt.System.BasicAux
+import Mt.System.Traced
 import Mt.Utils.List
 
 namespace Mt.System
@@ -20,100 +21,21 @@ open Utils
 -/
 def valid (s : System spec) : Prop :=
   ∀ s' : System spec, s.reduces_to_or_eq s' →
-  s'.panics = 0 ∧ spec.validate s'.reservations s'.state
+  s'.panics = 0 ∧ ∃ r, spec.validate r s'.state
 
 theorem fundamental_validation_theorem (s : System spec)
   (no_panics_yet : s.panics = 0)
-  (initial_valid : spec.validate s.reservations s.state)
+  (initial_valid : spec.validate IsReservation.empty s.state)
   (threads_valid : ∀ t, t ∈ s.threads → t.valid)
   : s.valid :=by
-  intro s' s_reduces_or_eq_to_s'
-  cases s_reduces_or_eq_to_s' <;> rename_i h
+  intro s' s_to_s'
+  cases s_to_s' <;> rename_i h
   . rw [<- h]
-    exact ⟨no_panics_yet, initial_valid⟩
+    exact ⟨no_panics_yet, IsReservation.empty, initial_valid⟩
   
-  suffices
-    (∀ t', t' ∈ s'.threads → t'.valid) ∧
-    s'.panics = 0 ∧ Spec.validate spec (reservations s') s'.state
-     from this.right
+  let traced := Traced.TracedSystem.mk_initial s
+  have traced_valid : traced.valid :=
+    Traced.TracedSystem.mk_initial.valid s no_panics_yet initial_valid threads_valid
 
-  induction h
-  . clear s s' ; rename_i s s' s_single_reduces_to_s'
-    
-    constructor
-    . -- show that threads are still valid after iteration
-      intro t' t'_def
-      apply Exists.elim <| single_reduce_elim s_single_reduces_to_s' t' t'_def
-      intro t h
-      apply Exists.elim h ; clear h ; intro state h
-      apply Or.elim h.right <;> (intro h')
-      . rw [<- h'] ; exact threads_valid t h.left
-      . have :=threads_valid t h.left
-        apply (System.decompose_reservation s h.left).elim
-        intro j ⟨_, decompose⟩
-        have :=(Thread.valid.def t).mp this (s.other_reservations j) s.state
-        rw [h'.right] at this
-        rw [<- decompose] at this
-        exact (this h'.left initial_valid).right
-
-    apply Exists.elim s_single_reduces_to_s'
-    intro i iteration ; rw [<- iteration]
-    simp only [iterate]
-    generalize t_def : List.get s.threads i = t
-    cases block_until : Thread.block_until t (reservations s)
-    next =>
-      . simp only [ite_false]
-        exact ⟨no_panics_yet, initial_valid⟩
-    constructor
-    . -- show s'.panic = 0, i.e. iterations do not panic
-      cases h : Thread.iterate t s.state <;> (simp only [] ; try assumption)
-      have :=List.get_in s.threads i ; rw [t_def] at this
-      have t_valid :=threads_valid t this
-
-      apply (System.decompose_reservation s this).elim
-      intro j ⟨_, decompose⟩
-
-      have :=(Thread.valid.def t).mp t_valid (s.other_reservations j) s.state
-      simp only [h, <- decompose] at this
-      exact (this block_until initial_valid).elim
-    . -- show that state/reservations are still valid after the iteration
-      have t_is_sthread :=List.get_in s.threads i ; rw [t_def] at t_is_sthread
-      have t_valid :=threads_valid t t_is_sthread
-      have decompose :=s.decompose_reservation' i t t_def.symm
-      simp only [ite_true]
-      cases h : Thread.iterate t s.state <;> (simp only [reservations])
-      . have :=(Thread.valid.def t).mp t_valid (s.other_reservations i) s.state
-        simp only [h, <- decompose] at this
-        
-        rename_i r state
-        rw [<- other_reservations]
-        have :=this block_until initial_valid
-        rw [this.right, IsReservation.toIsCommutative.comm,
-          IsReservation.empty_add] at this
-        exact this.left
-      . have :=(Thread.valid.def t).mp t_valid (s.other_reservations i) s.state
-        simp only [h, <- decompose] at this
-        exact (this block_until initial_valid).elim
-      . have :=(Thread.valid.def t).mp t_valid (s.other_reservations i) s.state
-        simp only [h, <- decompose] at this
-        
-        rename_i state cont
-        have :=this block_until initial_valid
-        
-        have temp :=System.decompose_reservation''
-          (List.set s.threads i.val cont)
-          ⟨i.val, calc
-            i.val < s.threads.length :=i.isLt
-            _ = (List.set s.threads i.val cont).length :=by simp
-          ⟩
-          cont
-          (Eq.symm <| List.get_of_set s.threads i.val cont _)
-        rw [temp] ; clear temp
-        simp only [List.erase_set]
-        rw [<- other_reservations]
-        exact this.left
-  . rename_i IHab IHbc
-    have :=IHab no_panics_yet initial_valid threads_valid
-    exact IHbc this.right.left this.right.right this.left
-
+  sorry
 end Mt.System
