Mt/System/Traced.lean
@@ -1,0 +1,204 @@
+import Mt.Thread.Traced
+import Mt.System.Basic
+import Mt.Utils.List
+
+namespace Mt.Traced
+
+structure TracedSystem (spec : Spec) where
+  state   : spec.State
+  threads : List (TracedThread spec)
+  panics  : Nat
+
+namespace TracedSystem
+
+variable {spec : Spec}
+
+local instance : IsReservation spec.Reservation :=spec.is_reservation
+
+def ThreadIndex (s : TracedSystem spec) : Type :=Fin s.threads.length
+def done (s : TracedSystem spec) : Bool :=s.threads.length = 0
+
+def iterate (s : TracedSystem spec) (idx : s.ThreadIndex) : Thread.IterationResult spec :=
+  (s.threads.get idx).iterate s.state
+
+def update_thread (s : TracedSystem spec) (idx : Nat) (state : spec.State)
+  (r : spec.Reservation) (cont : Thread spec) : TracedSystem spec :={
+  state
+  threads :=s.threads.set idx ⟨cont, r⟩
+  panics :=s.panics
+}
+
+def remove_thread (s : TracedSystem spec) (idx : Nat) (state : spec.State)
+  : TracedSystem spec :={
+  state
+  threads :=s.threads.eraseIdx idx
+  panics :=s.panics
+}
+
+def reservations (s : TracedSystem spec) : spec.Reservation :=
+  s.threads.foldl (λ env_r thread => env_r + thread.reservation) spec.is_reservation.empty
+
+def other_reservations (s : TracedSystem spec) (idx : Nat) : spec.Reservation :=
+  (s.threads.eraseIdx idx).foldl (λ env_r thread => env_r + thread.reservation) spec.is_reservation.empty
+
+theorem decompose_reservations (s : TracedSystem spec) (idx : s.ThreadIndex) :
+  s.reservations = s.other_reservations idx.val + (s.threads.get idx).reservation :=by
+  -- TODO
+  sorry
+
+structure valid (s : TracedSystem spec) : Prop where
+  no_panics_yet : s.panics = 0
+  currently_valid : spec.validate s.reservations s.state
+  threads_valid : ∀ t, t ∈ s.threads → t.valid 
+
+inductive reduces_to : TracedSystem spec -> TracedSystem spec -> Prop where
+| done {s : TracedSystem spec} (idx : s.ThreadIndex) {state}
+  (blocked_until : (s.threads.get idx).block_until s.state)
+  (iteration : s.iterate idx = Thread.IterationResult.Done state)
+  : s.reduces_to (s.remove_thread idx.val state)
+| running {s : TracedSystem spec} (idx : s.ThreadIndex) {state r cont}
+  (is_valid : spec.validate (s.other_reservations idx.val + r) state)
+  (cont_valid : cont.task.valid r cont.block_until λ _ r => r = IsReservation.empty)
+  : s.reduces_to (s.update_thread idx.val state r cont)
+| trans {a b c : TracedSystem spec} : a.reduces_to b -> b.reduces_to c -> a.reduces_to c
+
+theorem valid_forever {s s': TracedSystem spec} :
+  s.valid -> s.reduces_to s' -> s'.valid :=by
+  intro ⟨no_panics_yet, currently_valid, threads_valid⟩
+  intro s_to_s'
+  induction s_to_s' <;> clear s s'
+  . rename_i s idx state blocked_until iteration
+    constructor
+    . exact no_panics_yet
+    . let t :=s.threads.get idx
+      have t_valid :=threads_valid t (Utils.List.get_in ..)
+      conv at iteration =>
+        simp only [iterate]
+        arg 1 ; arg 1 ; change t
+      let env_r :=(s.remove_thread idx.val state).reservations
+      have decompose 
+        : s.reservations = env_r + _
+        :=s.decompose_reservations idx
+      rw [decompose] at currently_valid
+      have :=TracedThread.valid_elim t_valid env_r s.state blocked_until currently_valid
+      cases this
+      rename_i r t_valid
+      simp only [iteration] at t_valid
+      have := t_valid.left
+      rw [t_valid.right, IsReservation.toIsCommutative.comm, IsReservation.empty_add] at this
+      exact this
+    . intro t t_hyp
+      exact threads_valid t <| Utils.List.erase_subset s.threads idx.val t_hyp
+  . rename_i s idx state r cont is_valid cont_valid
+    constructor
+    . exact no_panics_yet
+    . let s' :=s.update_thread idx.val state r cont
+      have s'_def : s' = s.update_thread idx.val state r cont :=rfl
+      rw [<- s'_def]
+      let idx' : s'.ThreadIndex :=⟨idx.val, by calc
+        idx.val < s.threads.length :=idx.isLt
+              _ = s'.threads.length :=Eq.symm <| List.length_set ..⟩
+      have decompose :=s'.decompose_reservations idx'
+
+      conv at decompose =>
+        rhs
+        conv =>
+          arg 1
+          simp only [other_reservations, update_thread, Utils.List.erase_set]
+        conv =>
+          arg 2
+          simp only [update_thread, Utils.List.get_of_set]
+        
+      rw [decompose]
+      exact is_valid
+    . intro t' t'_hyp
+      cases Utils.List.set_subset s.threads idx.val _ t'_hyp
+      <;> rename_i t'_hyp
+      . rw [t'_hyp]
+        exact cont_valid
+      . exact threads_valid t' t'_hyp
+    
+  . rename_i a b _ _ _ IHab IHbc
+    have b_valid :=IHab no_panics_yet currently_valid threads_valid
+    exact IHbc b_valid.no_panics_yet b_valid.currently_valid b_valid.threads_valid
+
+def to_system (s : TracedSystem spec) : System spec :={
+  state := s.state
+  threads := s.threads.map λ ⟨t, _⟩ => t
+  panics := s.panics
+}
+
+def mk_initial (s : System spec) : TracedSystem spec :={
+  state := s.state
+  threads := s.threads.map λ t => ⟨t, IsReservation.empty⟩
+  panics := s.panics
+}
+
+theorem mk_initial.valid (s : System spec)
+  (no_panics_yet : s.panics = 0)
+  (initial_valid : spec.validate IsReservation.empty s.state)
+  (threads_valid : ∀ t, t ∈ s.threads → t.valid)
+  : (mk_initial s).valid :=by
+  constructor
+  . exact no_panics_yet
+  . simp only [mk_initial]
+    induction s.threads
+    . exact initial_valid
+    . rename_i head tail IH
+      simp only [List.map, Traced.TracedSystem.reservations, List.foldl, IsReservation.empty_add]
+      exact IH
+  . intro t t_hyp
+    simp only [mk_initial] at t_hyp
+    cases Utils.List.eq_of_in_map t_hyp
+    rename_i t_orig t_orig_hyp
+    rw [t_orig_hyp.right]
+    exact threads_valid t_orig t_orig_hyp.left
+
+theorem mk_initial.cancels_to_system {s : System spec} :
+  (mk_initial s).to_system = s :=by
+  simp only [mk_initial, to_system]
+  rw [System.mk.injEq]
+  constructor
+  . rfl
+  constructor
+  . induction s.threads
+    . rfl
+    . rename_i head tail IH
+      simp only [List.map]
+      rw [IH]
+  . rfl
+
+theorem reduces_by_iteration (s s' : System spec)
+  {idx : s.ThreadIndex}
+  {ts : TracedSystem spec}
+  (has_traced_system : s = ts.to_system)
+  (iteration : s.iterate idx = s')
+  (neq : s ≠ s')
+  : ∃ ts' : TracedSystem spec,
+    ts'.to_system = s' ∧ ts.reduces_to ts' :=by
+  simp only [System.iterate] at iteration
+  cases h : (s.threads.get idx).block_until s.state
+  <;> simp only [h, ite_true, ite_false] at iteration
+  . contradiction
+  have blocked_until :=h ; clear h
+  cases h : (s.threads.get idx).iterate s.state
+  <;> simp only [h] at iteration
+  . rename_i state
+    exists ts.remove_thread idx.val state
+    rw [<- iteration]
+    simp only [remove_thread]
+    constructor
+    . simp only [to_system, has_traced_system, System.mk.injEq, and_true, true_and]
+      -- TODO: Simple
+      sorry
+    . apply reduces_to.done ⟨idx.val, _⟩
+      . sorry
+      . simp only [iterate, TracedThread.iterate]
+        sorry
+      . sorry
+  . sorry
+  . sorry
+
+end TracedSystem
+
+end Mt.Traced
